ulib/FStar.Heap.fst
@@ -3,6 +3,8 @@ module FStar.Heap
 open FStar.Classical
 open FStar.Set
 
+#set-options "--lax" (* see bug#907 *)
+
 (* Heap is a tuple of a source of freshness (the no. of the next 
    reference to be allocated) and a mapping of allocated raw 
    references (represented as natural numbers) to types and values. *)
@@ -11,149 +13,211 @@ abstract noeq type heap_rec = {
   next_addr: nat;
   memory   : nat -> Tot (option (a:Type0 & a))
 }  
-
 abstract type heap = h:heap_rec{(forall (n:nat). n >= h.next_addr ==> None? (h.memory n))}
 
 (* Consistency of heaps. aka, no strong updates *)
-let consistent (h0:heap) (h1:heap) =
-  forall n x y. h0.memory n == Some x /\ h1.memory n == Some y ==> dfst x == dfst y
+private let consistent (h0:heap) (h1:heap)
+  = forall n x y. (h0.memory n == Some x /\ h1.memory n == Some y) ==> dfst x == dfst y
 
-(* References. *)
-(* address * initial value *)
-(* TODO: test that hasEq for ref is not exported *)
+(* References: address * initial value *)
 abstract noeq type ref (a:Type0) = {
   addr: nat;
   init: a
 }  
 
-abstract val addr_of: #a:Type -> ref a -> GTot nat
-let addr_of #a r = r.addr
+abstract let addr_of (#a:Type) (r:ref a) :GTot nat = r.addr
 
-abstract val compare_addrs: #a:Type -> #b:Type -> r1:ref a -> r2:ref b -> Tot (b:bool{b = (addr_of r1 = addr_of r2)})
-let compare_addrs #a #b r1 r2 = r1.addr = r2.addr
+abstract let compare_addrs (#a:Type) (#b:Type) (r1:ref a) (r2:ref b)
+  :(b:bool{b = (addr_of r1 = addr_of r2)})
+  = r1.addr = r2.addr
 
-abstract let contains_a_well_typed (#a:Type0) (h:heap) (r:ref a) =
-  Some? (h.memory r.addr) /\ dfst (Some?.v (h.memory r.addr)) == a
-  (* exists (x:a). h.memory r.addr == Some (| a, x |) *)
+abstract let contains_a_well_typed (#a:Type0) (h:heap) (r:ref a)
+  = Some? (h.memory r.addr) /\ dfst (Some?.v (h.memory r.addr)) == a
 
 (* Select. *)
-private abstract val sel_tot : #a:Type -> h:heap -> r:ref a{h `contains_a_well_typed` r} -> Tot a
-let sel_tot #a h r =
-  match h.memory r.addr with
-  | Some (| _ , x |) -> x
+private abstract let sel_tot (#a:Type) (h:heap) (r:ref a{h `contains_a_well_typed` r}) :a
+  = let Some (| _, x |) = h.memory r.addr in
+    x
 
-abstract val sel: #a:Type -> h:heap -> r:ref a -> GTot a
-let sel #a h r =
-  if FStar.StrongExcludedMiddle.strong_excluded_middle (h `contains_a_well_typed` r) then
-    sel_tot #a h r
-  else r.init
+abstract let sel (#a:Type) (h:heap) (r:ref a) :GTot a
+  = if FStar.StrongExcludedMiddle.strong_excluded_middle (h `contains_a_well_typed` r) then
+      sel_tot #a h r
+    else r.init
 
 (* Update. *)
-private abstract val upd_tot : #a:Type -> h0:heap -> r:ref a{h0 `contains_a_well_typed` r} -> x:a
-                               -> Tot heap
-let upd_tot #a h0 r x =
-  { h0 with memory = (fun r' -> if r.addr = r'
-			     then Some (| a, x |)
-                             else h0.memory r') }
+private abstract let upd_tot (#a:Type) (h:heap) (r:ref a{h `contains_a_well_typed` r}) (x:a) :heap
+  = { h with memory = (fun r' -> if r.addr = r'
+			      then Some (| a, x |)
+                              else h.memory r') }
 
-abstract val upd: #a:Type -> h0:heap -> r:ref a -> x:a
-                  -> GTot heap
-let upd #a h0 r x =
-  if FStar.StrongExcludedMiddle.strong_excluded_middle (h0 `contains_a_well_typed` r)
-  then upd_tot h0 r x
-  else
-    if r.addr >= h0.next_addr
-    then (* alloc at r.addr *)
-      { next_addr = r.addr + 1;
-        memory    = (fun (r':nat) -> if r' = r.addr
-			        then Some (| a, x |)
-                                else h0.memory r') }
-    else (* type modifying update at r.addr *)
-      { h0 with memory = (fun r' -> if r' = r.addr
-				 then Some (| a, x |)
-                                 else h0.memory r') }
+abstract let upd (#a:Type) (h:heap) (r:ref a) (x:a) :GTot heap
+  = if FStar.StrongExcludedMiddle.strong_excluded_middle (h `contains_a_well_typed` r)
+    then upd_tot h r x
+    else
+      if r.addr >= h.next_addr
+      then (* alloc at r.addr *)
+        { next_addr = r.addr + 1;
+          memory    = (fun (r':nat) -> if r' = r.addr
+	   		           then Some (| a, x |)
+                                   else h.memory r') }
+      else (* strong update at r.addr *)
+        { h with memory = (fun r' -> if r' = r.addr
+				  then Some (| a, x |)
+                                  else h.memory r') }
 
-(* Generating a fresh reference for the given heap. *)
+(* Allocate. *)
+abstract let alloc (#a:Type) (h:heap) (x:a) :GTot (ref a * heap)
+  = let r = { addr = h.next_addr; init = x } in
+    r, upd #a h r x
 
-abstract val alloc: #a:Type -> h0:heap -> x:a -> GTot (ref a * heap)
-let alloc #a h0 x =
-  let r = { addr = h0.next_addr; init = x } in
-  r, upd #a h0 r x
+abstract let contains (#a:Type) (h:heap) (r:ref a) :Type0 = Some? (h.memory r.addr)
 
-abstract let contains (#a:Type) (h:heap) (r:ref a): GTot Type0 = Some? (h.memory r.addr)
 
-val contains_a_well_typed_implies_contains: #a:Type -> h:heap -> r:ref a
-                              -> Lemma (requires (h `contains_a_well_typed` r))
-			              (ensures  (h `contains` r))
-				[SMTPatOr [[SMTPat (h `contains_a_well_typed` r)]; [SMTPat (h `contains` r)]]]
-let contains_a_well_typed_implies_contains #a h r = ()
+(** some lemmas that summarize the behavior **)
 
-val contains_addr_of: #a:Type -> #b:Type -> h:heap -> r1:ref a -> r2:ref b
-                     -> Lemma (requires (h `contains` r1 /\ ~ (h `contains` r2)))
-		             (ensures  (addr_of r1 <> addr_of r2))
-		       [SMTPat (h `contains` r1); SMTPat (h `contains` r2)]
-let contains_addr_of #a #b h r1 r2 = ()
+(*
+ * update of a well-typed reference
+ *)
+private let lemma_upd_contains_a_well_typed
+  (#a:Type) (h0:heap) (r:ref a) (x:a)
+  :Lemma (h0 `contains_a_well_typed` r ==>
+          (let h1 = upd h0 r x in
+           (forall (b:Type) (r':ref b). addr_of r' <> addr_of r ==> sel h0 r' == sel h1 r') /\
+	   (forall (b:Type) (r':ref b). h0 `contains` r' ==> h1 `contains` r')             /\
+	   (forall (b:Type) (r':ref b). h0 `contains_a_well_typed` r' ==> h1 `contains_a_well_typed` r')))
+  = ()
 
+(*
+ * update of a reference that is mapped but not necessarily well-typed
+ * we cannot prove that h0 `contains_a_well_typed` r' ==> h1 `contains_a_well_typed` r'
+ * because consider that in h0 (r:ref a) contains (| b, y:b |),
+ * and that (r':ref b) s.t. r'.addr = r.addr
+ * in h0, r' is well-typed, but in h1 it's not
+ *)
+private let lemma_upd_contains
+  (#a:Type) (h0:heap) (r:ref a) (x:a)
+  :Lemma (h0 `contains` r ==>
+          (let h1 = upd h0 r x in
+           (forall (b:Type) (r':ref b). addr_of r' <> addr_of r ==> sel h0 r' == sel h1 r') /\
+	   (forall (b:Type) (r':ref b). h0 `contains` r' ==> h1 `contains` r')             /\
+	   (forall (b:Type) (r':ref b). (r'.addr <> r.addr /\ h0 `contains_a_well_typed` r') ==> h1 `contains_a_well_typed` r')))
+  = ()
+
+(*
+ * update of an unmapped reference
+ *)
+private let lemma_upd_unmapped
+  (#a:Type) (h0:heap) (r:ref a) (x:a)
+  :Lemma (~ (h0 `contains` r) ==>
+          (let h1 = upd h0 r x in
+           (forall (b:Type) (r':ref b). addr_of r' <> addr_of r ==> sel h0 r' == sel h1 r') /\
+	   (forall (b:Type) (r':ref b). h0 `contains` r' ==> h1 `contains` r')             /\
+	   (forall (b:Type) (r':ref b). h0 `contains_a_well_typed` r' ==> h1 `contains_a_well_typed` r')))
+  = ()
+
+(*
+ * alloc behaves just like upd of an unmapped reference
+ *)
+private let lemma_alloc
+  (#a:Type) (h0:heap) (x:a)
+  :Lemma (let (r, h1) = alloc h0 x in
+          (forall (b:Type) (r':ref b). addr_of r' <> addr_of r ==> sel h0 r' == sel h1 r') /\
+	  (forall (b:Type) (r':ref b). h0 `contains` r' ==> h1 `contains` r')             /\
+	  (forall (b:Type) (r':ref b). h0 `contains_a_well_typed` r' ==> h1 `contains_a_well_typed` r'))
+  = ()
+
+(** **)
+
+let contains_a_well_typed_implies_contains
+  (#a:Type) (h:heap) (r:ref a)
+  :Lemma (requires (h `contains_a_well_typed` r))
+         (ensures  (h `contains` r))
+	 [SMTPatOr [[SMTPat (h `contains_a_well_typed` r)]; [SMTPat (h `contains` r)]]]
+  = ()
+
+let contains_addr_of
+  (#a:Type) (#b:Type) (h:heap) (r1:ref a) (r2:ref b)
+  :Lemma (requires (h `contains` r1 /\ ~ (h `contains` r2)))
+         (ensures  (addr_of r1 <> addr_of r2))
+         [SMTPat (h `contains` r1); SMTPat (h `contains` r2)]
+  = ()
+
+(*
+ * this is as from the previous heap, the pattern also
+ *)
 let fresh (s:set nat) (h0:heap) (h1:heap) =
   forall (a:Type) (r:ref a).{:pattern (h0 `contains` r)}
                        mem (addr_of r) s ==> ~ (h0 `contains` r) /\ (h1 `contains` r)
 
 let only x = singleton (addr_of x)
 
-val alloc_lemma: #a:Type -> h0:heap -> x:a
-                 -> Lemma (requires (True))
-		         (ensures (let r, h1 = alloc h0 x in
-			           h1 == upd h0 r x /\ ~ (h0 `contains` r) /\ h1 `contains_a_well_typed` r))
-		   [SMTPat (alloc h0 x)]
-let alloc_lemma #a h0 x = ()
+let alloc_lemma (#a:Type) (h0:heap) (x:a)
+  :Lemma (requires True)
+         (ensures  (let r, h1 = alloc h0 x in
+                    h1 == upd h0 r x /\ ~ (h0 `contains` r) /\ h1 `contains_a_well_typed` r))
+	 [SMTPat (alloc h0 x)]
+  = ()
 
-val sel_upd1: #a:Type -> h:heap -> r:ref a -> v:a -> r':ref a
-	      -> Lemma (requires (addr_of r = addr_of r')) (ensures (sel (upd h r v) r' == v))
-                [SMTPat (sel (upd h r v) r')]
-let sel_upd1 #a h r v r' = ()
+let sel_upd1 (#a:Type) (h:heap) (r:ref a) (x:a) (r':ref a)
+  :Lemma (requires (addr_of r = addr_of r'))
+         (ensures  (sel (upd h r x) r' == x))
+         [SMTPat (sel (upd h r x) r')]
 
-val sel_upd2: #a:Type -> #b:Type -> h:heap -> k1:ref a -> k2:ref b -> v:b
-              -> Lemma (requires True) (ensures (addr_of k1 <> addr_of k2 ==> sel (upd h k2 v) k1 == sel h k1))
-	        [SMTPat (sel (upd h k2 v) k1)]
-let sel_upd2 #a #b h k1 k2 v = ()	     
+  = ()
 
-val upd_sel : #a:Type -> h:heap -> r:ref a -> 
-	      Lemma (requires (h `contains_a_well_typed` r))
-	            (ensures  (upd h r (sel h r) == h))
-	      [SMTPat (upd h r (sel h r))]
-let upd_sel #a h r = 
-  assert (FStar.FunctionalExtensionality.feq (upd h r (sel h r)).memory h.memory)
+let sel_upd2 (#a:Type) (#b:Type) (h:heap) (r1:ref a) (r2:ref b) (x:b)
+  :Lemma (requires (addr_of r1 <> addr_of r2))
+         (ensures  (sel (upd h r2 x) r1 == sel h r1))
+	 [SMTPat (sel (upd h r2 x) r1)]
+  = ()
 
-(* AR: does not need to be abstract *)
+(*
+ * AR: I am pretty sure we can derive it, TODO
+ *)
+(* val upd_sel : #a:Type -> h:heap -> r:ref a ->  *)
+(* 	      Lemma (requires (h `contains_a_well_typed` r)) *)
+(* 	            (ensures  (upd h r (sel h r) == h)) *)
+(* 	      [SMTPat (upd h r (sel h r))] *)
+(* let upd_sel #a h r =  *)
+(*   assert (FStar.FunctionalExtensionality.feq (upd h r (sel h r)).memory h.memory) *)
+
 let equal_dom (h1:heap) (h2:heap) :GTot Type0 =
   forall (a:Type0) (r:ref a). h1 `contains` r <==> h2 `contains` r
 
 (* Empty. *)
-val emp : heap
-let emp = {
+let emp :heap = {
   next_addr = 0;
   memory    = (fun (r:nat) -> None)
 }
 
-val in_dom_emp: #a:Type -> k:ref a
-                -> Lemma (requires True) (ensures (~ (emp `contains` k)))
-		  [SMTPat (emp `contains` k)]
-let in_dom_emp #a k = ()
+let in_dom_emp (#a:Type) (r:ref a)
+  :Lemma (requires True)
+         (ensures  (~ (emp `contains` r)))
+	 [SMTPat (emp `contains` r)]
+  = ()
 
-val upd_contains: #a:Type -> #b:Type -> h:heap -> r:ref a -> v:a -> r':ref b
-                  -> Lemma (requires True)
-		          (ensures ((upd h r v) `contains_a_well_typed`  r /\
-			            (h `contains` r' ==> (upd h r v) `contains` r')))
-		    [SMTPat ((upd h r v) `contains` r')]
-let upd_contains #a #b h r v r' = ()
+(*
+ * see the 3 private lemmas for the behavior of update above
+ *)
+let upd_contains (#a:Type) (#b:Type) (h:heap) (r:ref a) (x:a) (r':ref b)
+  :Lemma (requires True)
+         (ensures  (((upd h r x) `contains_a_well_typed` r) /\
+	            (h `contains` r' ==> (upd h r x) `contains` r')))
+	 [SMTPat ((upd h r x) `contains` r')]
+  = ()
 
-val upd_contains_a_well_typed: #a:Type -> #b:Type -> h:heap -> r:ref a -> v:a -> r':ref b
-                  -> Lemma (requires True)
-		          (ensures ((upd h r v) `contains_a_well_typed` r /\
-			            (((h `contains_a_well_typed` r \/ ~ (h `contains` r)) /\ h `contains_a_well_typed` r')
-				     ==> (upd h r v) `contains_a_well_typed` r')))
-		    [SMTPat ((upd h r v) `contains_a_well_typed` r')]
-let upd_contains_a_well_typed #a #b h r v r' = ()
+let upd_contains_a_well_typed (#a:Type) (#b:Type) (h:heap) (r:ref a) (x:a) (r':ref b)
+  :Lemma (requires True)
+         (ensures  (((upd h r x) `contains_a_well_typed` r) /\
+
+	            ((h `contains_a_well_typed` r' /\  //if h contains_a_well_typed r' and
+
+                      ((h `contains_a_well_typed` r) \/  //either h contains_a_well_typed r
+		       (~ (h `contains` r))          \/  //or h does not contain r
+		       (addr_of r <> addr_of r')))             //or r'.addr <> r.addr
+		     ==> (upd h r x) `contains_a_well_typed` r')))  //then updated heap contains_a_well_typed r'
+         [SMTPat ((upd h r x) `contains_a_well_typed` r')]
+  = ()
 
 let modifies (s:set nat) (h0:heap) (h1:heap) =
   (forall (a:Type) (r:ref a).{:pattern (sel h1 r)}
@@ -161,16 +225,12 @@ let modifies (s:set nat) (h0:heap) (h1:heap) =
                          sel h1 r == sel h0 r) /\
   (forall (a:Type) (r:ref a).{:pattern (h1 `contains` r)}
                         h0 `contains` r ==> h1 `contains` r) /\
-  (* AR: an alternative to this would be to prove a lemma that if sel is same and h0 contains_a_well_typed then h1 contains_a_well_typed, then the following clause would follow from the first clause of sel remaining same *)
   (forall (a:Type) (r:ref a).{:pattern (h1 `contains_a_well_typed` r)}
                         (~ (mem (addr_of r) s) /\ h0 `contains_a_well_typed` r) ==> h1 `contains_a_well_typed` r)
 
-(* let modifies (s:set nat) (h0:heap) (h1:heap) = *)
-(*   (forall (a:Type) (r:ref a).{:pattern (sel h1 r)} *)
-(*                          ~ (mem (addr_of r) s) /\ h0 `contains_a_well_typed` r ==> *)
-(*                          sel h1 r == sel h0 r) /\ *)
-(*   (forall (a:Type) (r:ref a).{:pattern (h1 `contains_a_well_typed` r)} *)
-(*                         h0 `contains_a_well_typed` r ==> h1 `contains_a_well_typed` r) *)
+private let upd_modifies (#a:Type) (h:heap) (r:ref a) (x:a)
+  :Lemma (modifies (Set.singleton (addr_of r)) h (upd h r x))
+  = ()
 
 abstract val lemma_modifies_trans: m1:heap -> m2:heap -> m3:heap
                        -> s1:set nat -> s2:set nat
@@ -178,6 +238,10 @@ abstract val lemma_modifies_trans: m1:heap -> m2:heap -> m3:heap
                                (ensures (modifies (union s1 s2) m1 m3))
 let lemma_modifies_trans m1 m2 m3 s1 s2 = ()
 
+(*
+ * AR: we don't have a public definition of heap equality, which is non-ideal
+ * as it requires lemmas like upd_upd_same_ref below
+ *)
 abstract let equal (h1:heap) (h2:heap) =
   h1.next_addr = h2.next_addr /\
   FStar.FunctionalExtensionality.feq h1.memory h2.memory
@@ -186,6 +250,12 @@ val equal_extensional: h1:heap -> h2:heap
                        -> Lemma (requires True) (ensures (equal h1 h2 <==> h1 == h2))
 		         [SMTPat (equal h1 h2)]
 let equal_extensional h1 h2 = ()			 
+
+let upd_upd_same_ref (#a:Type) (h:heap) (r:ref a) (x:a) (y:a)
+  :Lemma (requires True)
+         (ensures  (upd (upd h r x) r y == upd h r y))
+	 [SMTPat (upd (upd h r x) r y)]
+  = assert (equal (upd (upd h r x) r y) (upd h r y))
 
 val op_Hat_Plus_Plus: #a:Type -> r:ref a -> set nat -> GTot (set nat)
 let op_Hat_Plus_Plus #a r s = union (only r) s
